FokkerChallenge/EnhancedCslib/Closedunderapp.lean
@@ -67,7 +67,7 @@ theorem closedunderapp_derive2 {P Q}
   | base h2 => exact h _ h2
   | app _ _ _ _ => grind
 
-@[simp, scoped grind]
+@[simp, scoped grind unfold]
 def ClosedUnderAppBool (P : Term String → Bool) : Term String → Bool
   | .app a b => ClosedUnderAppBool P a && ClosedUnderAppBool P b
   | a        => P a
